Wavelet.lean
@@ -2,7 +2,8 @@ import Wavelet.Semantics
 import Wavelet.Seq
 import Wavelet.Dataflow
 import Wavelet.Compile
+import Wavelet.Determinacy
 
 -- TODO: move these to better places
-import Wavelet.Determinacy
 import Wavelet.Typing
+import Wavelet.HighLevel
