Wavelet/HighLevel.lean
@@ -34,6 +34,30 @@ theorem sim_wt_prog
       ≲ᵣ (prog.semantics i).guard (opSpec.Guard (progSpec i))
   := by sorry
 
+/-- Final semantics of a sequential program when interpreted
+with a specific operator interpretation. -/
+abbrev Seq.Prog.semanticsᵢ
+  {Op : Type u₁} {χ : Type u₂} {V : Type u₃}
+  [Arity Op] [DecidableEq χ] [InterpConsts V]
+  [opInterp : OpInterp.{_, _, w} Op V]
+  {sigs : Sigs k}
+  {opSpec : Determinacy.OpSpec Op V T}
+  (prog : Prog (WithSpec Op opSpec) χ (V ⊕ T) (extendSigs sigs))
+  (i : Fin k) :
+    Semantics.{_, _, max u₁ u₂ u₃ w} Semantics.Empty V (sigs i).ι (sigs i).ω
+  := ((prog.semantics i).guard opSpec.TrivGuard).interpret opInterp
+
+/-- Final semantics of a dataflow program when interpreted
+with a specific operator interpretation. -/
+abbrev Dataflow.Proc.semanticsᵢ
+  {Op : Type u₁} {χ : Type u₂} {V : Type u₃}
+  [Arity Op] [DecidableEq χ] [InterpConsts V]
+  [opInterp : OpInterp.{_, _, w} Op V]
+  {opSpec : Determinacy.OpSpec Op V T}
+  (proc : Proc (WithSpec Op opSpec) χ (V ⊕ T) (m + 1) (n + 1)) :
+    Semantics.{_, _, max u₁ u₂ u₃ w} Semantics.Empty V m n
+  := (proc.semantics.guard opSpec.TrivGuard).interpret opInterp
+
 theorem compile_forward_sim
   [Arity Op] [PCM T] [PCM.Lawful T]
   [DecidableEq χ]
@@ -53,8 +77,49 @@ theorem compile_forward_sim
   · exact sim_wt_prog prog hwt
   apply IORestrictedSimilarity.trans
   · apply sim_guard
-    apply sim_compile_prog.{_, _, _, 0} (extendSigs sigs) prog ↑i (by omega) haff₁ haff₂
+    apply sim_compile_prog (extendSigs sigs) prog ↑i (by omega) haff₁ haff₂
   simp
   sorry
+
+theorem compile_strong_norm
+  {Op V T : Type u}
+  [Arity Op] [PCM T] [PCM.Lawful T]
+  [DecidableEq χ]
+  [InterpConsts V]
+  [opInterp : OpInterp.{_, _, w} Op V]
+  {sigs : Sigs k}
+  {opSpec : OpSpec Op V T}
+  {progSpec : ProgSpec Op V T sigs}
+  (prog : Prog (WithSpec Op opSpec) χ (V ⊕ T) (extendSigs sigs))
+  (hwt : ProgWithSpec.WellPermTyped progSpec prog)
+  (haff₁ : ∀ (i : Fin k), (prog i).AffineVar)
+  (haff₂ : prog.AffineInrOp)
+  (i : Fin k)
+  {args : Vector V (sigs i).ι}
+  {outputVals : Vector V (sigs i).ω}
+
+  {proc : Proc (WithSpec Op opSpec) (LinkName (ChanName χ)) (V ⊕ T) _ _}
+  (hcomp : proc = compileProg (extendSigs sigs) prog i)
+
+  {s s₁ s₂ : (prog.semanticsᵢ i).S}
+  {s' s₁' : proc.semanticsᵢ.S}
+  -- Same input values to both semantics
+  (hinputs : (prog.semanticsᵢ i).lts.Step (prog.semanticsᵢ i).init (.input args) s)
+  (hinputs' : proc.semanticsᵢ.lts.Step proc.semanticsᵢ.init (.input args) s')
+
+  -- There exists a terminating trace in the sequential semantics
+  -- that output `outputVals`.
+  (htrace : (prog.semanticsᵢ i).lts.TauStarN .τ k s s₁)
+  (hterm : (prog.semanticsᵢ i).lts.IsFinalFor (·.isSilent) s₁)
+  (houtput : (prog.semanticsᵢ i).lts.Step s₁ (.output outputVals) s₂)
+
+  (htrace' : proc.semanticsᵢ.lts.TauStarN .τ k' s' s₁') :
+    ∃ (s₁'' s₂' : proc.semanticsᵢ.S) (k'' : Nat),
+      k = k' + k'' ∧
+      proc.semanticsᵢ.lts.TauStarN .τ k'' s₁' s₁'' ∧
+      proc.semanticsᵢ.lts.IsFinalFor (·.isSilent) s₁'' ∧
+      proc.semanticsᵢ.lts.Step s₁'' (.output outputVals) s₂' ∧
+      s₂'.2 = s₂.2 -- Equal "memory" states
+  := sorry
 
 end Wavelet
